WIP

thys/examples/sorting/Sorting_Introsort.thy
@@ -1,9 +1,9 @@
 section \<open>Introsort (roughly libstdc++ version)\<close>
 theory Sorting_Introsort
 imports 
-  Sorting_Final_insertion_Sort Sorting_Heapsort Sorting_Log2 
+  Sorting_Final_insertion_Sort Sorting_Heapsort Sorting_Log2
   Sorting_Quicksort_Partition
-  Sorting_Strings
+ (* Sorting_Strings *)
 begin
 
 
@@ -12,11 +12,13 @@ context weak_ordering begin
 
   (* Assemble an introsort loop, using the partitioner and heap-sort *)  
   
-  definition introsort_aux4 :: "'a list \<Rightarrow> nat \<Rightarrow> nat \<Rightarrow> nat \<Rightarrow> 'a list nres" where "introsort_aux4 xs l h d \<equiv> RECT (\<lambda>introsort_aux (xs,l,h,d). doN {
+  definition introsort_aux4 :: "'a list \<Rightarrow> nat \<Rightarrow> nat \<Rightarrow> nat \<Rightarrow> ('a list, ecost) nrest"
+    where "introsort_aux4 xs l h d \<equiv> RECT' (\<lambda>introsort_aux (xs,l,h,d). doN {
     ASSERT (l\<le>h);
-    if h-l > is_threshold then doN {
-      if d=0 then
-        heapsort xs l h
+    lxs \<leftarrow> SPECc2 ''sub'' (-) h l; 
+    if\<^sub>N SPECc2 ''lt'' (<) is_threshold lxs then doN {
+      if\<^sub>N SPECc2 ''eq'' (=) d 0 then
+        heapsort2 xs l h
       else doN {
         (xs,m)\<leftarrow>partition_pivot xs l h;
         xs \<leftarrow> introsort_aux (xs,l,m,d-1);
@@ -29,30 +31,313 @@ context weak_ordering begin
   }) (xs,l,h,d)"
 
 
-  lemma introsort_aux4_refine: "introsort_aux4 xs l h d \<le> (introsort_aux3 xs l h d)"
-    unfolding introsort_aux4_def introsort_aux3_def
-    apply (rule refine_IdD)
-    apply (refine_rcg heapsort_correct' partition_pivot_correct)
+  definition heapsort_time' :: "_  \<Rightarrow> ecost" where
+    "heapsort_time' s = lift_acost (heapsort_lbc (s)) 
+          + cost ''add'' 1 + cost ''call'' (enat (s) + 2)
+          + cost ''icmp_slt'' (enat (s) + 1 + 1 + 1) + cost ''if'' (enat (s) + 1 + 3)
+          + cost ''sub'' (enat (s) + 2) + cost ''sift_down'' (enat (s))"
+
+  
+lemma heapsort_correct_h:
+  fixes xs\<^sub>0 :: "'a list"
+    assumes "l\<le>h\<^sub>0" "h\<^sub>0\<le>length xs\<^sub>0"
+    shows "heapsort xs\<^sub>0 l h\<^sub>0 \<le> SPEC (\<lambda>xs. slice_eq_mset l h\<^sub>0 xs xs\<^sub>0 \<and> sorted_wrt_lt (\<^bold><) (slice l h\<^sub>0 xs)) (\<lambda>_. heapsort_time' (h\<^sub>0-l))"
+  apply(rule order.trans[OF heapsort_correct[OF assms]])
+  apply(rule SPEC_leq_SPEC_I) apply simp
+  apply(auto simp: heapsort_time_def heapsort_time'_def heapsort_lbc_def lift_acost_propagate
+        lift_acost_cost)
+  apply sc_solve
+  apply safe by auto
+
+lemma wfR''_Rsd_a[simp]: "wfR'' (Rsd_a x)"
+  unfolding Rsd_a_def by auto
+
+  
+
+thm heapsort_correct' partition_pivot_correct
+
+text \<open>Here we assemble a Timerefinement from @{term heapsort_TR} and @{term TR_pp}.\<close>
+
+(* TODO *)
+definition "Tia43 \<equiv> TId(''slice_sort_p'':=
+        cost ''call'' (enat 10)
+         + cost ''if'' (enat 24) \<^cancel>\<open>
+         + cost ''sub'' c
+         + cost ''cmpo_v_idxs'' d
+         + cost ''mul'' e
+         + cost ''ofs_ptr'' f
+         + cost ''add'' g
+         + cost ''cmpo_idxs'' i
+         + cost ''udiv'' j
+         + cost ''add'' k
+         + cost ''icmp_slt'' m
+         + cost ''add'' n\<close>)"
+ 
+
+lemma cost_n_eq_TId_n: "cost n (1::enat) = TId n"
+  by(auto simp:  TId_def cost_def zero_acost_def less_eq_acost_def)
+
+lemma wfR''Tia43[simp]: "wfR'' (Tia43)"
+  by(auto simp: Tia43_def) 
+lemma spTia43[simp]: "struct_preserving (Tia43)"
+  by(auto simp: Tia43_def) 
+lemma pcTia43[simp]: 
+  "preserves_curr (Tia43) ''sub''"
+  "preserves_curr (Tia43) ''lt''"
+  "preserves_curr (Tia43) ''eq''"
+  by(auto simp: Tia43_def preserves_curr_def cost_n_eq_TId_n) 
+
+
+lemma yeah:
+  assumes "Discrete.log (h - l) \<ge> 1" "h-l \<ge> 1"
+  shows 
+  "timerefineA (heapsort_TR l h)  (cost ''slice_sort'' 1)
+      \<le> timerefineA (Tia43)
+       (cost ''slice_sort_p'' (enat ((h-l) * Discrete.log (h-l))))"
+  unfolding Tia43_def
+    unfolding heapsort_TR_def  singleton_heap_context.sift_down3_cost_def heapsort_time_def
+  unfolding pp_fun_upd pp_TId_absorbs_right 
+  apply(auto simp add: timerefineA_propagate)
+  unfolding Rsd_a_def heapsort_lbc_def 
+  apply(auto simp:   timerefineA_update_apply_same_cost' lift_acost_cost costmult_cost
+                lift_acost_propagate timerefineA_update_cost wfR''_TId intro!: wfR''_upd)
+  apply(subst timerefineA_propagate, auto)+
+  unfolding singleton_heap_context.sift_down3_cost_def  singleton_heap_context.E_sd3_l_def
+  apply(auto simp: costmult_cost costmult_add_distrib lift_acost_propagate lift_acost_cost)
+  apply(simp only: add.left_commute add.assoc cost_same_curr_left_add plus_enat_simps)
+  apply(simp add: timerefineA_update_apply_same_cost' costmult_cost costmult_add_distrib)
+  apply(simp only: add.left_commute)
+  apply sc_solve_debug
+  apply safe
+  subgoal (*if*)  apply(simp add: add_mult_distrib2 add_mult_distrib 
+              sc_solve_debug_def numeral_eq_enat plus_enat_simps one_enat_def times_enat_simps) 
+    apply(rule order.trans)
+     apply(rule add_mono[where b="7 * (h - l) * Discrete.log (h - l)"])
+    subgoal using assms by simp
+     apply(rule add_mono[where b="7 * (h - l) * Discrete.log (h - l)"])
+    subgoal apply simp apply(rule order.trans[where b="h-l"]) apply simp using assms by simp
+     apply(rule add_mono[where b="3 * (h - l) * Discrete.log (h - l)" and d="4 * (h - l) * Discrete.log (h - l)"])
+    subgoal   using assms by simp
+    subgoal using assms by simp
+    by linarith
+  subgoal (*call*) apply(simp add: add_mult_distrib2 add_mult_distrib 
+              sc_solve_debug_def  numeral_eq_enat plus_enat_simps one_enat_def times_enat_simps) 
+    apply(rule order.trans)
+    apply(subst Suc_eq_plus1_left)
+     apply(subst Suc_eq_plus1_left)
+     apply(rule add_mono[where b="1 * (h - l) * Discrete.log (h - l)"])
+    subgoal using assms by simp
+     apply(rule add_mono[where b="1 * (h - l) * Discrete.log (h - l)"])
+    subgoal using assms by simp
+     apply(rule add_mono[where b="1 * (h - l) * Discrete.log (h - l)"])
+    subgoal apply simp apply(rule order.trans[where b="h-l"]) apply simp using assms by simp
+     apply(rule add_mono[where b="1 * (h - l) * Discrete.log (h - l)"])
+    subgoal using assms by simp
+     apply(rule add_mono[where b="1 * (h - l) * Discrete.log (h - l)"])
+    subgoal using assms by simp
+     apply(rule add_mono[where b="1 * (h - l) * Discrete.log (h - l)"])
+    subgoal using assms by simp
+     apply(rule add_mono[where b="1 * (h - l) * Discrete.log (h - l)"])
+    subgoal apply simp apply(rule order.trans[where b="h-l"]) apply simp using assms by simp
+     apply(rule add_mono[where b="1 * (h - l) * Discrete.log (h - l)" and d="1 * (h - l) * Discrete.log (h - l)"])
+    subgoal apply simp apply(rule order.trans[where b="h-l"]) apply simp using assms by simp
+    subgoal   using assms by simp 
+    by linarith
+  sorry
+   
+  
+lemma yeah': (* i guess h-l must be \<ge> 2 *)
+  shows 
+  "(h-l)>1 \<Longrightarrow> timerefineA (heapsort_TR l h)  (cost ''slice_sort'' 1)
+      \<le> timerefineA (Tia43)
+       (cost ''slice_sort_p'' (enat ((h-l) * Discrete.log (h-l))))"
+  apply(rule yeah)
+  apply auto  
+  using Discrete.log.simps by auto  
+
+
+lemma heapsort_correct'': 
+  "\<lbrakk>(xs,xs')\<in>Id; (l,l')\<in>Id; (h,h')\<in>Id; lxs=(h'-l'); h'-l'>1\<rbrakk> \<Longrightarrow> heapsort2 xs l h \<le>
+      \<Down>Id (timerefine (Tia43) (slice_sort_specT (cost ''slice_sort_p'' (enat ((\<lambda>n. n * Discrete.log n) lxs))) (\<^bold><) xs' l' h'))"
+  apply(rule order.trans)
+   apply(rule heapsort_correct') apply auto [3] 
+  unfolding slice_sort_spec_def slice_sort_specT_def
+  apply(rule ASSERT_D3_leI)
+  apply(simp add: SPEC_timerefine_conv)
+  apply(rule SPEC_leq_SPEC_I)
+   apply simp 
+  apply(rule yeah') apply simp
+  done
+
+
+lemma
+  fixes R :: "_ \<Rightarrow> ('a, enat) acost"
+  assumes "x \<le> timerefine R y"
+    "R \<le> R'" "wfR'' R'"
+  shows "x \<le> timerefine R' y"
+  apply(rule order.trans)
+   apply(rule assms)
+  apply(rule timerefine_R_mono_wfR'') 
+   apply fact+ done
+
+lemma
+  fixes R :: "_ \<Rightarrow> ('a, enat) acost"
+  shows "R' \<le> sup R' R"
+  sorry
+
+
+lemma wfR''_supI:
+  fixes R:: "'b \<Rightarrow> ('c, enat) acost"
+  shows "wfR'' R \<Longrightarrow> wfR'' R' \<Longrightarrow> wfR'' (sup R R')"
+  unfolding wfR''_def
+  apply auto
+  subgoal premises prems for f
+    apply(rule finite_subset[where B="{s. the_acost (R s) f \<noteq> 0 \<or> the_acost (R' s) f \<noteq> 0}"])
+    subgoal apply auto  
+      by (simp add: sup_acost_def)    
+    subgoal
+      using prems[rule_format, of f]  
+      using finite_Collect_disjI by fastforce   
+    done
+  done
+
+lemma timerefine_supI:
+  fixes R :: "_ \<Rightarrow> ('a, enat) acost"
+  assumes "x \<le> timerefine R y"
+    "R \<le> R'" "wfR'' R'" "wfR'' R"
+  shows "x \<le> timerefine (sup R' R) y"
+  apply(rule order.trans)
+   apply(rule assms)
+  apply(rule timerefine_R_mono_wfR'') 
+  apply(rule wfR''_supI)
+   apply fact+ apply(rule sup_ge2) done
+
+
+lemma
+  fixes R :: "_ \<Rightarrow> ('a, enat) acost"
+  shows "sup TId R = R"
+  apply(rule ext)
+  apply simp
+  subgoal for x apply(cases "R x") unfolding TId_def sup_acost_def apply simp 
+    apply(rule ext) apply auto
+    oops
+
+
+lemma
+  fixes R :: "_ \<Rightarrow> ('b, enat) acost"
+  shows "sup (R(m:=x)) TId = (sup R TId)(m:=sup x (acostC (\<lambda>y. (if m=y then 1 else 0))))"
+  unfolding TId_def  by auto
+lemma
+  fixes R :: "_ \<Rightarrow> ('b, enat) acost"
+  shows "sup (R(m:=x)) TId = (sup R TId)(m:=sup x (acostC (\<lambda>y. (if m=y then 1 else 0))))"
+  unfolding TId_def  by auto
+
+lemma pullin_left:
+  fixes R :: "_ \<Rightarrow> ('b, enat) acost"
+  shows "sup (R(m:=x)) R' = (sup R R')(m:=sup x (R' m))"
+  apply(rule ext) by auto
+
+
+lemma "sup (TId(''a'':=cost ''n'' (2::enat))) (TId(''a'':=cost ''n'' 3, ''b'':=cost ''b'' 3)) = g"
+  apply(auto simp: pullin_left)
+  oops
+
+
+
+thm partition_pivot_correct 
+lemma partition_pivot_correct':
+  "\<lbrakk>(xs,xs')\<in>Id; (l,l')\<in>Id; (h,h')\<in>Id\<rbrakk> 
+  \<Longrightarrow> partition_pivot xs l h \<le> \<Down>Id (timerefine (Tia43) (partition3_spec xs' l' h'))"
+  sorry
+
+
+thm slice_sort_specT_def slice_sort_spec_def
+
+  lemma introsort_aux4_refine: "introsort_aux4 xs l h d \<le> \<Down>Id (timerefine (Tia43) ((introsort_aux3 (\<lambda>n. n * Discrete.log n) xs l h d)))"
+    unfolding introsort_aux4_def introsort_aux3_def 
+    supply conc_Id[simp del]
+    apply (refine_rcg RECT'_refine_t bindT_refine_conc_time_my_inres SPECc2_refine' MIf_refine
+            heapsort_correct'' partition_pivot_correct')
+    apply refine_mono
     apply refine_dref_type
-    apply simp_all 
+    apply (simp_all add: inres_SPECc2) 
     done
 
-  lemmas introsort_aux4_correct = order_trans[OF introsort_aux4_refine introsort_aux3_correct, THEN refine_IdI]
+lemma nlogn_mono:
+  "\<And>x y. x \<le> y \<Longrightarrow> x * Discrete.log x \<le> y * Discrete.log y"
+    apply(rule mult_mono) apply simp apply (rule log_mono[THEN monoD]) apply simp apply simp apply simp done
+lemma nlogn_sums: 
+  "a + b \<le> c \<Longrightarrow> a * Discrete.log a + b * Discrete.log b \<le> c * Discrete.log c"
+  apply(rule order.trans)
+   apply(rule add_mono[where b="a * Discrete.log c" and d="b * Discrete.log c"])
+  subgoal using log_mono[THEN monoD] by simp
+  subgoal using log_mono[THEN monoD] by simp
+  apply(subst add_mult_distrib[symmetric])
+  by simp
+ 
+thm introsort_aux3_correct 
 
+definition "bla d lxs = (pp (pp Tia43 (TId(''list_append'' := 0, ''list_length'' := cost ''sub'' 1))) (TId(''slice_part_sorted'' := introsort_aux_cost (\<lambda>n. n * Discrete.log n) (lxs, d))))"
+
+lemma "bla d lxs = gg"
+  unfolding bla_def 
+  apply(simp add: pp_fun_upd pp_TId_absorbs_right)
+  oops
+
+lemma introsort_aux4_correct: "introsort_aux4 xs l h d \<le> \<Down> Id (timerefine (bla d (h-l)) (slice_part_sorted_spec xs l h))"
+  apply(rule order.trans)
+   apply(rule introsort_aux4_refine)
+  apply(rule order.trans)
+   apply simp apply(rule timerefine_mono2)
+  apply simp
+   apply(rule introsort_aux3_correct)
+  subgoal apply(intro nlogn_mono) by simp
+  subgoal apply(intro nlogn_sums) by simp
+  apply (simp add: timerefine_iter2)
+  apply(subst timerefine_iter2)
+  subgoal sorry
+  subgoal by auto
+  unfolding bla_def apply simp
+  done
+ 
   definition "introsort4 xs l h \<equiv> doN {
     ASSERT(l\<le>h);
-    if h-l>1 then doN {
+    hml \<leftarrow> SPECc2 ''sub'' (-) h l;
+    if\<^sub>N SPECc2 ''lt'' (<) 1 hml then doN {
       xs \<leftarrow> introsort_aux4 xs l h (Discrete.log (h-l)*2);
       xs \<leftarrow> final_insertion_sort2 xs l h;
       RETURN xs
     } else RETURN xs
   }"  
 
-  lemma introsort4_refine: "introsort4 xs l h \<le> introsort3 xs l h"
-    unfolding introsort4_def introsort3_def
-    apply (rule refine_IdD)
-    apply (refine_rcg introsort_aux4_correct final_insertion_sort2_correct[THEN refine_IdI])
-    by auto
+lemma wfR''_bla[simp]: " wfR'' (bla d xs)"
+  unfolding bla_def
+  by(auto simp add:  pp_fun_upd pp_TId_absorbs_right intro!: wfR''_upd) 
+
+thm introsort_aux4_correct
+
+thm final_insertion_sort2_correct
+
+  lemma final_insertion_sort2_correct': 
+    assumes [simplified, simp]: "(xs',xs)\<in>Id" "(l',l)\<in>Id" "(h',h)\<in>Id"   
+    shows "final_insertion_sort2 xs' l' h' \<le> \<Down>Id (timerefine (bla (Discrete.log (h-l)*2) (h-l)) (final_sort_spec xs l h))"
+    sorry (* TODO *)
+
+lemma pc_bla[simp]:
+  "preserves_curr (bla d hl) ''sub''"
+  "preserves_curr (bla d hl) ''lt''"
+  by(auto simp: pcTia43[unfolded preserves_curr_def] pp_fun_upd pp_TId_absorbs_right  bla_def preserves_curr_def cost_n_eq_TId_n) 
+
+lemma sp_bla[simp]:
+  "struct_preserving (bla d hl)"
+  by (auto simp: pp_fun_upd pp_TId_absorbs_right  bla_def intro!: struct_preserving_upd_I)  
+
+  lemma introsort4_refine: "introsort4 xs l h \<le> \<Down>Id (timerefine (bla (Discrete.log (h-l)*2) (h-l)) (introsort3 xs l h))"
+    unfolding introsort4_def introsort3_def 
+    supply conc_Id[simp del]
+    apply (refine_rcg SPECc2_refine' bindT_refine_conc_time_my_inres MIf_refine introsort_aux4_correct final_insertion_sort2_correct' )
+    apply refine_dref_type
+    by auto   
 
   lemmas introsort4_correct = order_trans[OF introsort4_refine introsort3_correct]
 
@@ -77,6 +362,62 @@ qed
 
 
 context sort_impl_context begin
+
+
+thm partition_pivot2_refines heapsort3_refine
+
+definition "TR5 = sup E_mmtf E45"
+
+lemma TR_sup_Tid: "sup TId TId = TId"
+  by simp
+
+
+lemma pullin_right:
+  fixes R :: "_ \<Rightarrow> ('b, enat) acost"
+  shows "sup R' (R(m:=x)) = (sup R' R)(m:=sup (R' m) x)"
+  apply(rule ext) by auto
+
+lemma "TR5 = E45"
+  unfolding TR5_def  
+  apply(simp add: pullin_left pullin_right cost_n_eq_TId_n[symmetric])
+  oops
+
+
+  definition introsort_aux5 :: "'a list \<Rightarrow> nat \<Rightarrow> nat \<Rightarrow> nat \<Rightarrow> ('a list, ecost) nrest"
+    where "introsort_aux5 xs l h d \<equiv> RECT' (\<lambda>introsort_aux (xs,l,h,d). doN {
+    ASSERT (l\<le>h);
+    lxs \<leftarrow> SPECc2 ''sub'' (-) h l; 
+    if\<^sub>N SPECc2 ''lt'' (<) is_threshold lxs then doN {
+      if\<^sub>N SPECc2 ''eq'' (=) d 0 then
+        heapsort3 xs l h
+      else doN {
+        (xs,m)\<leftarrow>partition_pivot2 xs l h;
+        xs \<leftarrow> introsort_aux (xs,l,m,d-1);
+        xs \<leftarrow> introsort_aux (xs,m,h,d-1);
+        RETURN xs
+      }
+    }
+    else
+      RETURN xs
+  }) (xs,l,h,d)"
+
+
+lemma sp_E_mmtf[simp]: "struct_preserving E_mmtf"
+  sorry
+
+  lemma introsort_aux5_refine: "introsort_aux5 xs l h d \<le> \<Down>Id (timerefine (E_mmtf) ((introsort_aux4 xs l h d)))"
+    unfolding introsort_aux4_def introsort_aux5_def 
+    supply conc_Id[simp del]
+    apply (refine_rcg RECT'_refine_t bindT_refine_conc_time_my_inres SPECc2_refine' MIf_refine
+            heapsort3_refine partition_pivot2_refines)
+    apply refine_mono
+    apply refine_dref_type
+    apply (simp_all add: inres_SPECc2) 
+    done
+
+
+
+
 
 sepref_register introsort_aux4
 sepref_def introsort_aux_impl is "uncurry3 (PR_CONST introsort_aux4)" :: "(arr_assn)\<^sup>d *\<^sub>a size_assn\<^sup>k *\<^sub>a size_assn\<^sup>k *\<^sub>a size_assn\<^sup>k \<rightarrow>\<^sub>a arr_assn"
@@ -104,7 +445,7 @@ theorem introsort_impl_correct: "(uncurry2 introsort_impl, uncurry2 (slice_sort_
 end
 
 
-
+(*
 context parameterized_weak_ordering begin
   (* TODO: Move *)
   lemmas heapsort_param_refine'[refine] = heapsort_param_refine[unfolded heapsort1.refine[OF WO.weak_ordering_axioms, symmetric]]
@@ -205,7 +546,7 @@ lemma introsort_param_impl_correct: "(uncurry3 introsort_param_impl, uncurry3 (P
   using introsort_param_impl.refine[FCOMP introsort_param_correct'] .
   
 end
-
+*)
 
 
 end
